Continue work on lazy

STerm.v
@@ -5,7 +5,7 @@ Require Import Misc.
 Require Import Psatz.
 Require Import Star.
 Require Import Coq.Logic.Eqdep_dec.
-
+Require Import FEnv.
 
 Definition renaming := list nat.
 Fixpoint renv (L : renaming) (n : nat) : nat :=
@@ -779,34 +779,73 @@ Proof.
 Qed.
 
 
+Inductive closed_at : term -> nat -> Prop :=
+| closed_at_var : forall n k, n < k -> closed_at (var n) k
+| closed_at_app : forall t1 t2 k, closed_at t1 k -> closed_at t2 k -> closed_at (app t1 t2) k
+| closed_at_abs : forall t k, closed_at t (S k) -> closed_at (abs t) k.
 
 Inductive clo :=
-| mkclo : term -> list clo -> clo.
+| clo_var : nat -> clo
+| clo_term : term -> list clo -> clo.
 
+Inductive clo_closed_at : clo -> nat -> Prop :=
+| cc_var : forall n k, n < k -> clo_closed_at (clo_var n) k
+| cc_term : forall t l k, closed_at t (length l) -> (forall c, c \in l -> clo_closed_at c k) -> clo_closed_at (clo_term t l) k.
+
+(*
 Fixpoint shift_clo (c : clo) : clo :=
   match c with
   | mkclo t l => mkclo (ren_term (shiftn (length l)) t) (map shift_clo l)
   end.
+ *)
 
 Definition read_env (e : list term) :=
   fun n => match nth_error e n with Some u => u | None => var (n - length e) end.
 
-Fixpoint read_clo (c : clo) : term :=
+Fixpoint read_clo (k : nat) (c : clo) : term :=
   match c with
-  | mkclo t l =>
-    let nl := map read_clo l in
+  | clo_var n => var (k - 1 - n)
+  | clo_term t l =>
+    let nl := map (read_clo k) l in
     subst (read_env nl) t
   end.
 
-Fixpoint clo_ind2 (P : clo -> Prop) (H : forall t l, Forall P l -> P (mkclo t l)) (c : clo) : P c :=
+Fixpoint clo_ind2 (P : clo -> Prop) (Hvar : forall n, P (clo_var n)) (Hterm : forall t l, Forall P l -> P (clo_term t l)) (c : clo) : P c :=
   match c with
-  | mkclo t l => H t l ((fix H2 (l : _) : Forall P l :=
-              match l with
-              | nil => @Forall_nil _ _
-              | cons c l => @Forall_cons _ _ c l (clo_ind2 P H c) (H2 l)
-              end) l)
+  | clo_var n => Hvar n
+  | clo_term t l => Hterm t l ((fix H (l : _) : Forall P l :=
+                                 match l with
+                                 | nil => @Forall_nil _ _
+                                 | cons c l => @Forall_cons _ _ c l (clo_ind2 P Hvar Hterm c) (H l)
+                                 end) l)
   end.
 
+Lemma subst_closed_at_ext :
+  forall t k us1 us2, closed_at t k -> (forall n, n < k -> us1 n = us2 n) -> subst us1 t = subst us2 t.
+Proof.
+  induction t; intros k us1 us2 Hclosed Hext; inversion Hclosed; subst; simpl.
+  - apply Hext. assumption.
+  - f_equal. eapply IHt; [eassumption|].
+    intros [|n] Hn; simpl in *; [reflexivity|].
+    unfold comp. f_equal. apply Hext. lia.
+  - f_equal; [eapply IHt1 | eapply IHt2]; eassumption.
+Qed.
+
+Lemma read_shift_clo :
+  forall c k, clo_closed_at c k -> read_clo (S k) c = ren_term (plus_ren 1) (read_clo k c).
+Proof.
+  induction c using clo_ind2; intros k Hccat; inversion Hccat; subst; simpl.
+  - f_equal. lia.
+  - rewrite ren_subst. eapply subst_closed_at_ext; [eassumption|].
+    intros n Hn. unfold comp, read_env.
+    rewrite !nth_error_map.
+    destruct nth_error as [u|] eqn:Hu; [|apply nth_error_None in Hu; lia].
+    assert (u \in l) by (eapply nth_error_In; eassumption).
+    rewrite Forall_forall in H; apply H; [eassumption|].
+    apply H4; assumption.
+Qed.
+
+(*
 Lemma read_shift_clo :
   forall c, read_clo (shift_clo c) = ren_term (plus_ren 1) (read_clo c).
 Proof.
@@ -822,18 +861,30 @@ Proof.
     replace (nth_error l _) with (@None clo) by (symmetry; apply nth_error_None; lia).
     unfold ren_term. rewrite plus_ren_correct. f_equal. lia.
 Qed.
-
+*)
 Inductive valE : deep_flag -> Type :=
 | valEs_nf : nfval -> valE shallow
 | valEs_abs : term -> list clo -> valE shallow
 | valEd_nf : nfval_or_lam -> valE deep.
 
+(*
 Definition read_valE {df} (v : valE df) : val df :=
   match v with
   | valEs_nf v => vals_nf v
   | valEs_abs t v => vals_abs (subst (scons (var 0) (comp (ren_term (plus_ren 1)) (read_env (map read_clo v)))) t)
   | valEd_nf v => vald_nf v
   end.
+*)
+
+Definition read_valE {df} (k : nat) (v : valE df) : val df :=
+  match v with
+  | valEs_nf v => vals_nf v
+  | valEs_abs t v =>
+  (* vals_abs (subst (scons (var 0) (comp (ren_term (plus_ren 1)) (read_env (map read_clo v)))) t) *)
+    vals_abs (subst (scons (var 0) (read_env (map (read_clo (S k)) v))) t)
+  | valEd_nf v => vald_nf v
+  end.
+
 
 Definition valE_nf {df} v : valE df :=
   match df with
@@ -842,7 +893,7 @@ Definition valE_nf {df} v : valE df :=
   end.
 
 Lemma read_valE_nf :
-  forall df v, read_valE (@valE_nf df v) = val_nf v.
+  forall df k v, read_valE k (@valE_nf df v) = val_nf v.
 Proof.
   intros [|] v; simpl; reflexivity.
 Qed.
@@ -857,51 +908,70 @@ Arguments extE_term {df} _.
 Arguments extE_app {df} _ _.
 Arguments extE_appnf {df} _ _.
 
+Definition valE_closed {df} k (v : valE df) :=
+  match v with
+  | valEs_abs t l => closed_at t (S (length l)) /\ (forall c, c \in l -> clo_closed_at c k)
+  | _ => True
+  end.
+
+Definition outE_closed {df} k (o : out (valE df)) :=
+  match o with
+  | out_div => True
+  | out_ret v => valE_closed k v
+  end.
+
+Inductive extE_closed_at : forall {df}, extE df -> nat -> nat -> Prop :=
+| extE_term_closed : forall df t k1 k2, closed_at t k1 -> extE_closed_at (@extE_term df t) k1 k2
+| extE_app_closed : forall df o t k1 k2, closed_at t k1 -> outE_closed k2 o -> extE_closed_at (@extE_app df o t) k1 k2
+| extE_appnf_closed : forall df v o k1 k2, outE_closed k2 o -> extE_closed_at (@extE_appnf df v o) k1 k2
+| extEd_abs_closed : forall o k1 k2, outE_closed (S k2) o -> extE_closed_at (extEd_abs o) k1 k2.
+
 Definition out_map {A B : Type} (f : A -> B) (o : out A) : out B :=
   match o with
   | out_ret x => out_ret (f x)
   | out_div => out_div
   end.
 
-Definition read_extE {df} env (e : extE df) : ext df :=
+Definition read_extE {df} k env (e : extE df) : ext df :=
   match e with
-  | extE_term t => ext_term (read_clo (mkclo t env))
-  | extE_app o1 t2 => ext_app (out_map read_valE o1) (read_clo (mkclo t2 env))
-  | extE_appnf v1 o2 => ext_appnf v1 (out_map read_valE o2)
-  | extEd_abs o => extd_abs (out_map read_valE o)
+  | extE_term t => ext_term (read_clo k (clo_term t env))
+  | extE_app o1 t2 => ext_app (out_map (read_valE k) o1) (read_clo k (clo_term t2 env))
+  | extE_appnf v1 o2 => ext_appnf v1 (out_map (read_valE k) o2)
+  | extEd_abs o => extd_abs (out_map (read_valE (S k)) o)
   end.
 
-Inductive redE : forall df, list clo -> extE df -> out (valE df) -> Prop :=
-| redE_var_bound : forall df env n t2 env2 o,
-    nth_error env n = Some (mkclo t2 env2) ->
-    redE df env2 (extE_term t2) o ->
-    redE df env (extE_term (var n)) o
-| redE_var_free : forall df env n,
-    nth_error env n = None ->
-    redE df env (extE_term (var n)) (out_ret (valE_nf (nvar (n - length env))))
-| redE_abs_shallow : forall t env,
-    redE shallow env (extE_term (abs t)) (out_ret (valEs_abs t env))
-| redE_abs_deep : forall t env o1 o2,
-    redE deep (mkclo (var 0) nil :: map shift_clo env) (extE_term (ren_term (shiftn (S (length env))) t)) o1 ->
-    redE deep env (extEd_abs o1) o2 ->
-    redE deep env (extE_term (abs t)) o2
-| redE_abs1_abort : forall env, redE deep env (extEd_abs out_div) out_div
-| redE_abs1 : forall env v, redE deep env (extEd_abs (out_ret (valEd_nf v))) (out_ret (valEd_nf (nlam v)))
-| redE_app : forall df env t1 o1 t2 o2,
-    redE shallow env (extE_term t1) o1 ->
-    redE df env (extE_app o1 t2) o2 ->
-    redE df env (extE_term (app t1 t2)) o2
-| redE_app1_abort : forall df env t2, redE df env (extE_app out_div t2) out_div
-| redE_app1_nf : forall df env v o1 t2 o2,
-    redE deep env (extE_term t2) o1 ->
-    redE df env (extE_appnf v o1) o2 ->
-    redE df env (extE_app (out_ret (valEs_nf v)) t2) o2
-| redE_app1_abs : forall df env env2 t1 t2 o,
-    redE df (mkclo t2 env :: env2) (extE_term t1) o ->
-    redE df env (extE_app (out_ret (valEs_abs t1 env2)) t2) o
-| redE_appnf_abort : forall df env v, redE df env (extE_appnf v out_div) out_div
-| redE_appnf : forall df env v1 v2, redE df env (extE_appnf v1 (out_ret (valEd_nf v2))) (out_ret (valE_nf (napp v1 v2))).
+Inductive redE : forall df, nat -> list clo -> extE df -> out (valE df) -> Prop :=
+| redE_var_bound : forall df k env n t2 env2 o,
+    nth_error env n = Some (clo_term t2 env2) ->
+    redE df k env2 (extE_term t2) o ->
+    redE df k env (extE_term (var n)) o
+| redE_var_free : forall df k env n p,
+    nth_error env n = Some (clo_var p) ->
+    redE df k env (extE_term (var n)) (out_ret (valE_nf (nvar (k - 1 - p))))
+| redE_abs_shallow : forall t k env,
+    redE shallow k env (extE_term (abs t)) (out_ret (valEs_abs t env))
+| redE_abs_deep : forall t k env o1 o2,
+    redE deep (S k) (clo_var k :: env) (extE_term t) o1 ->
+    redE deep k env (extEd_abs o1) o2 ->
+    redE deep k env (extE_term (abs t)) o2
+| redE_abs1_abort : forall k env, redE deep k env (extEd_abs out_div) out_div
+| redE_abs1 : forall k env v, redE deep k env (extEd_abs (out_ret (valEd_nf v))) (out_ret (valEd_nf (nlam v)))
+| redE_app : forall df k env t1 o1 t2 o2,
+    redE shallow k env (extE_term t1) o1 ->
+    redE df k env (extE_app o1 t2) o2 ->
+    redE df k env (extE_term (app t1 t2)) o2
+| redE_app1_abort : forall df k env t2, redE df k env (extE_app out_div t2) out_div
+| redE_app1_nf : forall df k env v o1 t2 o2,
+    redE deep k env (extE_term t2) o1 ->
+    redE df k env (extE_appnf v o1) o2 ->
+    redE df k env (extE_app (out_ret (valEs_nf v)) t2) o2
+| redE_app1_abs : forall df k env env2 t1 t2 o,
+    redE df k (match t2 with var n => match nth_error env n with Some c => c | _ => clo_term t2 env end | _ => clo_term t2 env end :: env2) (extE_term t1) o ->
+    redE df k env (extE_app (out_ret (valEs_abs t1 env2)) t2) o
+| redE_appnf_abort : forall df k env v, redE df k env (extE_appnf v out_div) out_div
+| redE_appnf : forall df k env v1 v2, redE df k env (extE_appnf v1 (out_ret (valEd_nf v2))) (out_ret (valE_nf (napp v1 v2))).
 
+(*
 CoInductive coredE : forall df, list clo -> extE df -> out (valE df) -> Prop :=
 | coredE_var_bound : forall df env n t2 env2 o,
     nth_error env n = Some (mkclo t2 env2) ->
@@ -917,7 +987,8 @@ CoInductive coredE : forall df, list clo -> extE df -> out (valE df) -> Prop :=
     coredE deep env (extEd_abs o1) o2 ->
     coredE deep env (extE_term (abs t)) o2
 | coredE_abs1_abort : forall env, coredE deep env (extEd_abs out_div) out_div
-| coredE_abs1 : forall env v, coredE deep env (extEd_abs (out_ret (valEd_nf v))) (out_ret (valEd_nf (nlam v)))
+| coredE_abs1 : forall env v, coredE deep env (ext				isIntNum = false;
+Ed_abs (out_ret (valEd_nf v))) (out_ret (valEd_nf (nlam v)))
 | coredE_app : forall df env t1 o1 t2 o2,
     coredE shallow env (extE_term t1) o1 ->
     coredE df env (extE_app o1 t2) o2 ->
@@ -932,165 +1003,472 @@ CoInductive coredE : forall df, list clo -> extE df -> out (valE df) -> Prop :=
     coredE df env (extE_app (out_ret (valEs_abs t1 env2)) t2) o
 | coredE_appnf_abort : forall df env v, coredE df env (extE_appnf v out_div) out_div
 | coredE_appnf : forall df env v1 v2, coredE df env (extE_appnf v1 (out_ret (valEd_nf v2))) (out_ret (valE_nf (napp v1 v2))).
-
+*)
 Arguments nth_error : simpl nomatch.
-Lemma redE_red :
-  forall df env e o, redE df env e o -> red df (read_extE env e) (out_map read_valE o).
+
+Lemma valE_nf_closed :
+  forall df v k, valE_closed k (@valE_nf df v).
 Proof.
-  intros df env e o H. induction H; simpl in *.
-  - unfold read_env. rewrite nth_error_map, H. assumption.
-  - unfold read_env. rewrite nth_error_map, H, map_length, read_valE_nf. constructor.
+  intros [|]; simpl; tauto.
+Qed.
+
+Lemma clo_closed_at_mono :
+  forall c k1, clo_closed_at c k1 -> forall k2, k1 < k2 -> clo_closed_at c k2.
+Proof.
+  induction c using clo_ind2; intros k1 Hck1 k2 Hk12; inversion Hck1; subst; constructor.
+  - lia.
+  - assumption.
+  - rewrite Forall_forall in H. intros c Hc. eapply H; [assumption| |eassumption].
+    apply H4; assumption.
+Qed.
+
+Lemma redE_closed :
+  forall df k env e o, (forall c, c \in env -> clo_closed_at c k) -> extE_closed_at e (length env) k -> redE df k env e o -> outE_closed k o.
+Proof.
+  intros df k env e o Henv He H. induction H; simpl in *; inversion He; subst.
+  - apply nth_error_In, Henv in H. inversion H; subst.
+    apply IHredE; [|constructor]; assumption.
+  - apply valE_nf_closed.
+  - split; [|assumption].
+    inversion H1; subst. assumption.
+  - apply IHredE2; [assumption|]. constructor.
+    apply IHredE1; [|constructor; inversion H3; subst; assumption].
+    intros c [<- | Hc]; [constructor; lia|].
+    eapply clo_closed_at_mono; [apply Henv; assumption|]. lia.
+  - tauto.
+  - tauto.
+  - apply IHredE2; [assumption|]. constructor; [inversion H3; subst; assumption|].
+    apply IHredE1; [assumption|]. constructor; inversion H3; subst; assumption.
+  - tauto.
+  - apply IHredE2; [assumption|]. constructor.
+    apply IHredE1; [assumption|]. constructor. assumption.
+  - apply IHredE; [intros c [<- | Hc]|].
+    + destruct t2; try (constructor; assumption).
+      destruct nth_error eqn:Hu; [|constructor; assumption].
+      eapply Henv, nth_error_In; eassumption.
+    + simpl in *. apply H6. assumption.
+    + simpl in *. constructor. apply H6.
+  - tauto.
+  - apply valE_nf_closed.
+Qed.
+
+Lemma redE_red :
+  forall df k env e o, (forall c, c \in env -> clo_closed_at c k) -> extE_closed_at e (length env) k -> redE df k env e o -> red df (read_extE k env e) (out_map (read_valE k) o).
+Proof.
+  intros df k env e o Henv He H. induction H; simpl in *; inversion He; subst.
+  - unfold read_env. rewrite nth_error_map, H.
+    apply nth_error_In, Henv in H. inversion H; subst.
+    apply IHredE; [assumption|]. constructor. assumption.
+  - unfold read_env. rewrite nth_error_map, H, read_valE_nf. constructor.
+  - inversion H1; subst.
+    erewrite subst_closed_at_ext; [constructor|eassumption|].
+    intros [|n] Hn; [reflexivity|]. unfold comp, read_env; simpl.
+    rewrite !nth_error_map; destruct nth_error as [u|] eqn:Hu.
+    + rewrite read_shift_clo; [reflexivity|]. apply Henv. eapply nth_error_In; eassumption.
+    + apply nth_error_None in Hu. lia.
+  - econstructor; [|apply IHredE2; [assumption|constructor]].
+    erewrite subst_closed_at_ext.
+    + apply IHredE1; [|constructor; inversion H3; assumption].
+      intros c [<- | Hc]; [constructor; lia|].
+      eapply clo_closed_at_mono; [apply Henv; assumption|]. lia.
+    + inversion H3; eassumption.
+    + intros [|n] Hn; unfold comp, read_env; simpl; [f_equal; lia|].
+      rewrite !nth_error_map; destruct nth_error as [u|] eqn:Hu.
+      * rewrite read_shift_clo; [|eapply Henv, nth_error_In; eassumption].
+        reflexivity.
+      * apply nth_error_None in Hu; lia.
+    + eapply redE_closed; [| |eassumption].
+      * intros c [<- | Hc]; [constructor; lia|].
+        eapply clo_closed_at_mono; [apply Henv; assumption|]. lia.
+      * constructor. inversion H3; simpl; subst. assumption.
   - constructor.
-  - rewrite subst_ren in IHredE1.
-    econstructor; [|eassumption].
-    erewrite subst_ext; [eassumption|].
-    intros [|n]; unfold comp, read_env; [reflexivity|].
-    unfold ren. rewrite renv_shiftn.
-    destruct le_lt_dec; simpl; rewrite !nth_error_map, !map_length; destruct nth_error as [u|] eqn:Hu.
-    + assert (Hu2 : nth_error env n <> None) by congruence; rewrite nth_error_Some in Hu2; lia.
-    + assert (HSn : nth_error env (S n) = None) by (apply nth_error_None; lia); rewrite HSn.
-      unfold ren_term. simpl. destruct (length env); f_equal; simpl; lia.
-    + rewrite read_shift_clo. reflexivity.
-    + rewrite nth_error_None in Hu. lia.
   - constructor.
+  - econstructor; [apply IHredE1|apply IHredE2]; try assumption; constructor; try (inversion H3; assumption).
+    eapply redE_closed; [| |eassumption]; [assumption|]. constructor. inversion H3; assumption.
   - constructor.
-  - econstructor; eassumption.
-  - constructor.
-  - econstructor; eassumption.
+  - econstructor; [apply IHredE1|apply IHredE2]; try assumption; constructor; try assumption.
+    eapply redE_closed; [| |eassumption]; [assumption|]. constructor. assumption.
   - econstructor.
     unfold subst1. rewrite subst_subst.
-    erewrite subst_ext; [eassumption|].
-    unfold comp, read_env.
-    intros [|n]; simpl.
-    + reflexivity.
-    + rewrite subst_ren; unfold comp; simpl.
-      erewrite subst_ext; [apply subst_id|]; intros; f_equal; lia.
+    erewrite subst_closed_at_ext; [apply IHredE| |].
+    + intros c [<- | Hc]; [|simpl in H6; apply H6; assumption].
+      destruct t2; try (constructor; assumption).
+      destruct nth_error eqn:Hu; [|constructor; assumption].
+      eapply Henv, nth_error_In; eassumption.
+    + simpl in H6. constructor. apply H6.
+    + simpl in H6. apply H6.
+    + unfold comp, read_env.
+      intros [|n] Hn; simpl.
+      * destruct t2; try reflexivity. simpl.
+        rewrite nth_error_map. destruct nth_error eqn:Hu; [|apply nth_error_None in Hu; inversion H3; subst; lia].
+        reflexivity.
+      * rewrite !nth_error_map; destruct nth_error as [u|] eqn:Hu; [|apply nth_error_None in Hu; lia].
+        rewrite read_shift_clo by (simpl in H6; eapply H6, nth_error_In; eassumption).
+        rewrite subst_ren; unfold comp; simpl.
+        erewrite subst_ext; [apply subst_id|]; intros; f_equal; lia.
   - constructor.
   - rewrite read_valE_nf. constructor.
 Qed.
 
-(*
-Inductive redE : forall df, list clo -> extE df -> out (valE df) -> Prop :=
-| redE_var_bound : forall df env n t2 env2 o,
-    nth_error env n = Some (mkclo t2 env2) ->
-    redE df env2 (extE_term t2) o ->
-    redE df env (extE_term (var n)) o
-| redE_var_free : forall df env n,
-    nth_error env n = None ->
-    redE df env (extE_term (var n)) (out_ret (valE_nf (nvar (n - length env))))
-| redE_abs_shallow : forall t env,
-    redE shallow env (extE_term (abs t)) (out_ret (valEs_abs t env))
-| redE_abs_deep : forall t env o1 o2,
-    redE deep (mkclo (var 0) nil :: map shift_clo env) (extE_term (ren_term (shiftn (S (length env))) t)) o1 ->
-    redE deep env (extEd_abs o1) o2 ->
-    redE deep env (extE_term (abs t)) o2
-| redE_abs1_abort : forall env, redE deep env (extEd_abs out_div) out_div
-| redE_abs1 : forall env v, redE deep env (extEd_abs (out_ret (valEd_nf v))) (out_ret (valEd_nf (nlam v)))
-| redE_app : forall df env t1 o1 t2 o2,
-    redE shallow env (extE_term t1) o1 ->
-    redE df env (extE_app o1 t2) o2 ->
-    redE df env (extE_term (app t1 t2)) o2
-| redE_app1_abort : forall df env t2, redE df env (extE_app out_div t2) out_div
-| redE_app1_nf : forall df env v o1 t2 o2,
-    redE deep env (extE_term t2) o1 ->
-    redE df env (extE_appnf v o1) o2 ->
-    redE df env (extE_app (out_ret (valEs_nf v)) t2) o2
-| redE_app1_abs : forall df env env2 t1 t2 o,
-    redE df (mkclo t2 env :: env2) (extE_term t1) o ->
-    redE df env (extE_app (out_ret (valEs_abs t1 env2)) t2) o
-| redE_appnf_abort : forall df env v, redE df env (extE_appnf v out_div) out_div
-| redE_appnf : forall df env v1 v2, redE df env (extE_appnf v1 (out_ret (valEd_nf v2))) (out_ret (valE_nf (napp v1 v2))).
-*)
 
 
-
-
-
-
-
-
-
-
-
-
-
-
-
-
-
-
-
-
-
-
-
-
-
-
-
-
-
-
-
-
-
-
-Definition ext_shallow_to_deep (e : ext shallow) : ext deep :=
-  match e return ext deep with
-  | ext_term t => ext_term t
-  | ext_app o1 t2 => ext_app o1 t2
-  | ext_appnf v1 o2 => ext_appnf v1 o2
-  | extd_abs t => extd_abs t
+Definition extE_shallow_to_deep (e : extE shallow) : extE deep :=
+  match e return extE deep with
+  | extE_term t => extE_term t
+  | extE_app o1 t2 => extE_app o1 t2
+  | extE_appnf v1 o2 => extE_appnf v1 o2
+  | extEd_abs t => extEd_abs t
   end.
 
-Lemma red_shallow_deep_val_aux :
-  forall df e o,
-    red df e o -> forall (p : df = shallow) v, (match p in _ = df return out (val df) with eq_refl => o end) = out_ret (vals_nf v) ->
-    red deep (ext_shallow_to_deep (match p in _ = df return ext df with eq_refl => e end)) (out_ret (vald_nf (nval v))).
+Lemma redE_shallow_deep_val_aux :
+  forall df k env e o,
+    redE df k env e o -> forall (p : df = shallow) v, (match p in _ = df return out (valE df) with eq_refl => o end) = out_ret (valEs_nf v) ->
+    redE deep k env (extE_shallow_to_deep (match p in _ = df return extE df with eq_refl => e end)) (out_ret (valEd_nf (nval v))).
 Proof.
-  intros df e o H.
-  induction H; try destruct df; intros p; try discriminate p; rewrite (UIP_dec deep_flag_eq_dec p eq_refl);
+  intros df k env e o H.
+  induction H; try destruct df; intros Hdf; try discriminate Hdf; rewrite (UIP_dec deep_flag_eq_dec Hdf eq_refl);
     intros nv Ho; try discriminate Ho; simpl.
-  - injection Ho as Ho; subst. constructor.
+  - subst. econstructor; [eassumption|]. eapply (IHredE eq_refl). reflexivity.
+  - injection Ho as Ho; subst. apply (redE_var_free deep). assumption.
   - econstructor; [eassumption|].
-    eapply (IHred2 eq_refl). assumption.
+    eapply (IHredE2 eq_refl). assumption.
   - econstructor; [eassumption|].
-    eapply (IHred2 eq_refl). assumption.
+    eapply (IHredE2 eq_refl). assumption.
   - econstructor.
-    eapply (IHred eq_refl). eassumption.
+    eapply (IHredE eq_refl). eassumption.
   - injection Ho as Ho; subst. constructor.
 Qed.
 
-Lemma red_shallow_deep_val :
-  forall e v, red shallow e (out_ret (vals_nf v)) ->
-         red deep (ext_shallow_to_deep e) (out_ret (vald_nf (nval v))).
+Lemma redE_shallow_deep_val :
+  forall k env e v, redE shallow k env e (out_ret (valEs_nf v)) ->
+         redE deep k env (extE_shallow_to_deep e) (out_ret (valEd_nf (nval v))).
 Proof.
-  intros e v H.
-  exact (red_shallow_deep_val_aux shallow e _ H eq_refl v eq_refl).
+  intros k env e v H.
+  exact (redE_shallow_deep_val_aux shallow k env e _ H eq_refl v eq_refl).
 Qed.
 
-Lemma red_shallow_deep_abs_aux :
-  forall df e o,
-    red df e o -> forall (p : df = shallow) t, (match p in _ = df return out (val df) with eq_refl => o end) = out_ret (vals_abs t) ->
-    forall o2, red deep (ext_term (abs t)) o2 -> red deep (ext_shallow_to_deep (match p in _ = df return ext df with eq_refl => e end)) o2.
+Lemma redE_shallow_deep_abs_aux :
+  forall df k env e o,
+    redE df k env e o -> forall (p : df = shallow) t env2, (match p in _ = df return out (valE df) with eq_refl => o end) = out_ret (valEs_abs t env2) ->
+    forall o2, redE deep k env2 (extE_term (abs t)) o2 -> redE deep k env (extE_shallow_to_deep (match p in _ = df return extE df with eq_refl => e end)) o2.
 Proof.
-  intros df e o H.
-  induction H; try destruct df; intros p; try discriminate p; rewrite (UIP_dec deep_flag_eq_dec p eq_refl);
-    intros nt Ho; try discriminate Ho; simpl.
+  intros df k env e o H.
+  induction H; try destruct df; intros Hdf; try discriminate Hdf; rewrite (UIP_dec deep_flag_eq_dec Hdf eq_refl);
+    intros nt nenv Ho; try discriminate Ho; simpl.
+  - subst. intros o2 Ho2. econstructor; [eassumption|]. eapply (IHredE eq_refl); [reflexivity|eassumption].
   - injection Ho as Ho; subst. intros; assumption.
-  - intros o3. specialize (IHred2 eq_refl nt Ho o3). simpl in IHred2.
-    intros Hred. econstructor; [eassumption|]. apply IHred2; assumption.
-  - intros o3. specialize (IHred2 eq_refl nt Ho o3). simpl in IHred2.
-    intros Hred. econstructor; [eassumption|]. apply IHred2; assumption.
-  - intros o3. specialize (IHred eq_refl nt Ho o3). simpl in IHred.
-    intros Hred. constructor. apply IHred; assumption.
+  - intros o3. specialize (IHredE2 eq_refl nt nenv Ho o3). simpl in IHredE2.
+    intros HredE. econstructor; [eassumption|]. apply IHredE2; assumption.
+  - intros o3. specialize (IHredE2 eq_refl nt nenv Ho o3). simpl in IHredE2.
+    intros HredE. econstructor; [eassumption|]. apply IHredE2; assumption.
+  - intros o3. specialize (IHredE eq_refl nt nenv Ho o3). simpl in IHredE.
+    intros HredE. constructor. apply IHredE; assumption.
 Qed.
 
-Lemma red_shallow_deep_abs :
-  forall e t,
-    red shallow e (out_ret (vals_abs t)) ->
-    forall o, red deep (ext_term (abs t)) o -> red deep (ext_shallow_to_deep e) o.
+Lemma redE_shallow_deep_abs :
+  forall k env env2 e t,
+    redE shallow k env e (out_ret (valEs_abs t env2)) ->
+    forall o, redE deep k env2 (extE_term (abs t)) o -> redE deep k env (extE_shallow_to_deep e) o.
 Proof.
-  intros e t H.
-  exact (red_shallow_deep_abs_aux shallow e _ H eq_refl t eq_refl).
+  intros k env env2 e t H.
+  exact (redE_shallow_deep_abs_aux shallow k env e _ H eq_refl t env2 eq_refl).
 Qed.
+
+
+
+
+
+
+
+Inductive eiM :=
+| eiM_lazy : term -> list freevar -> eiM
+| eiM_abs1 : term -> list freevar -> eiM
+| eiM_abs2 : term -> list freevar -> nfval_or_lam -> eiM
+| eiM_val : nfval -> eiM.
+Definition memM := list (freevar * eiM).
+
+Inductive read_eiM (env : memM) : freevar -> clo -> nat -> Prop :=
+| read_eiM_lazy : forall x t yvs k,
+    env_find env x = Some (eiM_lazy t (map fst yvs)) ->
+    (forall y v, In (y, v) yvs -> read_eiM env y v k) ->
+    read_eiM env x (clo_term t (map snd yvs)) k
+| read_eiM_abs1 : forall x t yvs u ws k,
+    env_find env x = Some (eiM_abs1 t (map fst yvs)) ->
+    (forall y v, In (y, v) yvs -> read_eiM env y v k) ->
+    redE shallow k ws (extE_term u) (out_ret (valEs_abs t (map snd yvs))) ->
+    read_eiM env x (clo_term u ws) k
+| read_eiM_abs2 : forall x t yvs u ws v k,
+    env_find env x = Some (eiM_abs2 t (map fst yvs) v) ->
+    (forall y v, In (y, v) yvs -> read_eiM env y v k) ->
+    redE shallow k ws (extE_term u) (out_ret (valEs_abs t (map snd yvs))) ->
+    redE deep k ws (extE_term u) (out_ret (valEd_nf (nlam v))) ->
+    read_eiM env x (clo_term u ws) k
+| read_eiM_val : forall x u ws v k,
+    env_find env x = Some (eiM_val v) ->
+    redE shallow k ws (extE_term u) (out_ret (valEs_nf v)) ->
+    read_eiM env x (clo_term u ws) k
+| read_eiM_var : forall x p k,
+    p < k -> env_find env x = Some (eiM_val (nvar (k - 1 - p))) ->
+    read_eiM env x (clo_var p) k.
+
+Inductive valM : deep_flag -> Type :=
+| valMs_nf : nfval -> valM shallow
+| valMs_abs : term -> list freevar -> valM shallow
+| valMd_nf : nfval_or_lam -> valM deep.
+
+Inductive read_valM : forall {df}, nat -> memM -> valM df -> valE df -> Prop :=
+| read_valMs_nf : forall env k v, @read_valM shallow k env (valMs_nf v) (valEs_nf v)
+| read_valMs_abs : forall env k t xvs,
+    (forall x v, In (x, v) xvs -> read_eiM env x v k) ->
+    @read_valM shallow k env (valMs_abs t (map fst xvs)) (valEs_abs t (map snd xvs))
+| read_valMd_nf : forall env k v, @read_valM deep k env (valMd_nf v) (valEd_nf v).
+
+Definition valM_nf {df} v : valM df :=
+  match df with
+  | shallow => valMs_nf v
+  | deep => valMd_nf (nval v)
+  end.
+
+Lemma read_valM_nf :
+  forall df env k v, read_valM k env (@valM_nf df v) (valE_nf v).
+Proof.
+  intros [|] env k v; simpl; constructor.
+Qed.
+
+
+Inductive outM t m :=
+| outM_ret : t -> m -> outM t m
+| outM_div : outM t m.
+
+Arguments outM_ret {t} {m} _ _.
+Arguments outM_div {t} {m}.
+
+Inductive extM : deep_flag -> Type :=
+| extM_term : forall df, term -> extM df
+| extM_app : forall df, outM (valM shallow) memM -> term -> extM df
+| extM_appnf : forall df, nfval -> outM (valM deep) memM -> extM df
+| extMd_abs : outM (valM deep) memM -> extM deep.
+
+Arguments extM_term {df} _.
+Arguments extM_app {df} _ _.
+Arguments extM_appnf {df} _ _.
+
+Definition compat_memM (m1 m2 : memM) :=
+  forall x c k, read_eiM m1 x c k -> read_eiM m2 x c k.
+
+Inductive read_outM : forall df, nat -> memM -> outM (valM df) memM -> out (valE df) -> Prop :=
+| read_outM_div : forall df m k, read_outM df k m outM_div out_div
+| read_outM_ret : forall df m1 m2 k v1 v2, compat_memM m1 m2 -> read_valM k m2 v1 v2 -> read_outM df k m1 (outM_ret v1 m2) (out_ret v2).
+
+Inductive read_extM : forall df, memM -> nat -> extM df -> extE df -> Prop :=
+| read_extM_term : forall df m k t, read_extM df m k (extM_term t) (extE_term t)
+| read_extM_app : forall df m k o1 o2 t, read_outM shallow k m o1 o2 -> read_extM df m k (extM_app o1 t) (extE_app o2 t)
+| read_extM_appnf : forall df m k v o1 o2, read_outM deep k m o1 o2 -> read_extM df m k (extM_appnf v o1) (extE_appnf v o2)
+| read_extMd_abs : forall m k o1 o2, read_outM deep k m o1 o2 -> read_extM deep m k (extMd_abs o1) (extEd_abs o2).
+
+Inductive redM : forall df, nat -> list freevar -> extM df -> memM -> outM (valM df) memM -> Prop :=
+| redM_var_val : forall df k n env m x v,
+    nth_error env n = Some x ->
+    env_find m x = Some (eiM_val v) ->
+    redM df k env (extM_term (var n)) m (outM_ret (valM_nf v) m)
+(* | redM_var_bound : forall df env n t2 env2 o,
+    nth_error env n = Some (mkclo t2 env2) ->
+    redM df env2 (extM_term t2) o ->
+    redM df env (extM_term (var n)) o
+| redM_var_free : forall df env n,
+    nth_error env n = None ->
+    redM df env (extM_term (var n)) (out_ret (valM_nf (nvar (n - length env)))) *)
+| redM_abs_shallow : forall k t env m,
+    redM shallow k env (extM_term (abs t)) m (outM_ret (valMs_abs t env) m)
+(*| redM_abs_deep : forall t env m o1 o2,
+    redM deep (mkclo (var 0) nil :: map shift_clo env) (extM_term (ren_term (shiftn (S (length env))) t)) m o1 ->
+    redM deep env (extMd_abs o1) m o2 ->
+    redM deep env (extM_term (abs t)) m o2 *)
+| redM_abs1_abort : forall k env m, redM deep k env (extMd_abs outM_div) m outM_div
+| redM_abs1 : forall k env m1 m2 v, redM deep k env (extMd_abs (outM_ret (valMd_nf v) m2)) m1 (outM_ret (valMd_nf (nlam v)) m2)
+| redM_app : forall df k env m t1 o1 t2 o2,
+    redM shallow k env (extM_term t1) m o1 ->
+    redM df k env (extM_app o1 t2) m o2 ->
+    redM df k env (extM_term (app t1 t2)) m o2
+| redM_app1_abort : forall df k env m t2, redM df k env (extM_app outM_div t2) m outM_div
+| redM_app1_nf : forall df k env m1 m2 v o1 t2 o2,
+    redM deep k env (extM_term t2) m2 o1 ->
+    redM df k env (extM_appnf v o1) m2 o2 ->
+    redM df k env (extM_app (outM_ret (valMs_nf v) m2) t2) m1 o2
+| redM_app1_abs : forall df k env env2 env3 m1 m2 m3 a t1 t2 o,
+    a = match t2 with var n => nth_error env n | _ => None end ->
+    match a with Some x => env3 = x :: env2 /\ m3 = m2 | None => exists x, env_find m2 x = None /\ env3 = x :: env2 /\ m3 = (x, eiM_lazy t2 env) :: m2 end ->
+    redM df k env3 (extM_term t1) m3 o ->
+    redM df k env (extM_app (outM_ret (valMs_abs t1 env2) m2) t2) m1 o
+| redM_appnf_abort : forall df k env m v, redM df k env (extM_appnf v outM_div) m outM_div
+| redM_appnf : forall df k env m1 m2 v1 v2,
+    redM df k env (extM_appnf v1 (outM_ret (valMd_nf v2) m2)) m1 (outM_ret (valM_nf (napp v1 v2)) m2).
+
+(*
+Inductive redE : forall df, nat -> list clo -> extE df -> out (valE df) -> Prop :=
+| redE_var_bound : forall df k env n t2 env2 o,
+    nth_error env n = Some (clo_term t2 env2) ->
+    redE df k env2 (extE_term t2) o ->
+    redE df k env (extE_term (var n)) o
+| redE_var_free : forall df k env n p,
+    nth_error env n = Some (clo_var p) ->
+    redE df k env (extE_term (var n)) (out_ret (valE_nf (nvar (k - 1 - p))))
+| redE_abs_shallow : forall t k env,
+    redE shallow k env (extE_term (abs t)) (out_ret (valEs_abs t env))
+| redE_abs_deep : forall t k env o1 o2,
+    redE deep (S k) (clo_var k :: env) (extE_term t) o1 ->
+    redE deep k env (extEd_abs o1) o2 ->
+    redE deep k env (extE_term (abs t)) o2
+| redE_abs1_abort : forall k env, redE deep k env (extEd_abs out_div) out_div
+| redE_abs1 : forall k env v, redE deep k env (extEd_abs (out_ret (valEd_nf v))) (out_ret (valEd_nf (nlam v)))
+| redE_app : forall df k env t1 o1 t2 o2,
+    redE shallow k env (extE_term t1) o1 ->
+    redE df k env (extE_app o1 t2) o2 ->
+    redE df k env (extE_term (app t1 t2)) o2
+| redE_app1_abort : forall df k env t2, redE df k env (extE_app out_div t2) out_div
+| redE_app1_nf : forall df k env v o1 t2 o2,
+    redE deep k env (extE_term t2) o1 ->
+    redE df k env (extE_appnf v o1) o2 ->
+    redE df k env (extE_app (out_ret (valEs_nf v)) t2) o2
+| redE_app1_abs : forall df k env env2 t1 t2 o,
+    redE df k (match t2 with var n => match nth_error env n with Some c => c | _ => clo_term t2 env end | _ => clo_term t2 env end :: env2) (extE_term t1) o ->
+    redE df k env (extE_app (out_ret (valEs_abs t1 env2)) t2) o
+| redE_appnf_abort : forall df k env v, redE df k env (extE_appnf v out_div) out_div
+| redE_appnf : forall df k env v1 v2, redE df k env (extE_appnf v1 (out_ret (valEd_nf v2))) (out_ret (valE_nf (napp v1 v2))).
+
+*)
+
+Lemma compat_memM_refl :
+  forall m, compat_memM m m.
+Proof.
+  intros m x c k H. exact H.
+Qed.
+
+Lemma compat_memM_trans :
+  forall m1 m2 m3, compat_memM m1 m2 -> compat_memM m2 m3 -> compat_memM m1 m3.
+Proof.
+  intros m1 m2 m3 H1 H2 x c k H. apply H2. apply H1. assumption.
+Qed.
+
+Lemma compat_memM_read_outM :
+  forall df k m1 m2 o1 o2, compat_memM m1 m2 -> read_outM df k m2 o1 o2 -> read_outM df k m1 o1 o2.
+Proof.
+  intros df k m1 m2 o1 o2 H1 H2. inversion H2; unexistT; subst; simpl in *.
+  - constructor.
+  - constructor; [|assumption].
+    eapply compat_memM_trans; eassumption.
+Qed.
+
+
+Lemma redM_redE :
+  forall df k env e m o,
+    redM df k env e m o ->
+    forall cenv e2, env = map fst cenv -> (forall x c, (x, c) \in cenv -> read_eiM m x c k) ->
+               read_extM df m k e e2 ->
+               exists o2, redE df k (map snd cenv) e2 o2 /\ read_outM df k m o o2.
+Proof.
+  intros df k env e m o H. induction H; intros cenv e2 Henv1 Henv2 Hread; inversion Hread; unexistT; subst; simpl in *.
+  - rewrite nth_error_map in H. destruct nth_error as [u|] eqn:Hu; [|congruence].
+    injection H; intros; subst. destruct u as [x c]; simpl in *; subst.
+    assert (Hu2 := Henv2 x c ltac:(eapply nth_error_In; eassumption)).
+    inversion Hu2; rewrite H0 in *; subst; try congruence.
+    + injection H1; intros; subst. exists (out_ret (valE_nf v0)).
+      split.
+      * econstructor; [rewrite nth_error_map, Hu; reflexivity|].
+        destruct df; simpl; [assumption|].
+        eapply redE_shallow_deep_val in H2. assumption.
+      * constructor; [apply compat_memM_refl|]. apply read_valM_nf.
+    + injection H2; intros; subst. exists (out_ret (valE_nf (nvar (k - 1 - p)))).
+      split.
+      * eapply redE_var_free. rewrite nth_error_map, Hu. reflexivity.
+      * constructor; [apply compat_memM_refl|]. apply read_valM_nf.
+  - eexists; split; [econstructor|].
+    constructor; [apply compat_memM_refl|].
+    constructor. assumption.
+  - inversion H3; unexistT; subst; simpl in *.
+    eexists; split; [econstructor|]. constructor.
+  - inversion H3; unexistT; subst; simpl in *.
+    inversion H7; unexistT; subst; simpl in *.
+    eexists; split; [econstructor|].
+    constructor; [assumption|]. constructor.
+  - specialize (IHredM1 cenv (extE_term t1)).
+    destruct IHredM1 as (o3 & HredE1 & Ho3); [reflexivity|assumption|constructor|].
+    specialize (IHredM2 cenv (extE_app o3 t2)).
+    destruct IHredM2 as (o4 & HredE2 & Ho4); [reflexivity|assumption|constructor; assumption|].
+    exists o4. split; [econstructor; eassumption|assumption].
+  - inversion H3; unexistT; subst; simpl in *.
+    eexists; split; [econstructor|]. constructor.
+  - inversion H5; unexistT; subst; simpl in *.
+    inversion H9; unexistT; subst; simpl in *.
+    specialize (IHredM1 cenv (extE_term t2)).
+    destruct IHredM1 as (o3 & HredE1 & Ho3); [reflexivity|intros; apply H8; apply Henv2; assumption|constructor|].
+    specialize (IHredM2 cenv (extE_appnf v o3)).
+    destruct IHredM2 as (o4 & HredE2 & Ho4); [reflexivity|intros; apply H8; apply Henv2; assumption|constructor; assumption|].
+    exists o4. split; [econstructor; eassumption|].
+    eapply compat_memM_read_outM; eassumption.
+  - inversion H6; unexistT; subst; simpl in *.
+    inversion H9; unexistT; subst; simpl in *.
+    match goal with [ _ : match ?a with Some _ => _ | None => _ end |- _ ] => destruct a as [x|] eqn:Ha end.
+    + destruct H0 as [Henv3 Hm3]; subst.
+      destruct t2; try congruence.
+      rewrite nth_error_map in Ha. destruct nth_error as [xv|] eqn:Hxv; [|congruence]; subst.
+      injection Ha as <-.
+      specialize (IHredM (xv :: xvs) (extE_term t1)).
+      destruct IHredM as (o2 & HredE & Ho2).
+      * reflexivity.
+      * intros x c [-> | Hxc]; [|apply H7; assumption].
+        eapply H8, Henv2, nth_error_In; eassumption.
+      * constructor.
+      * exists o2. split; [|eapply compat_memM_read_outM; eassumption].
+        constructor. rewrite nth_error_map, Hxv; assumption.
+    + destruct H0 as (x & Hx & Henv3 & Hm3); subst.
+      assert (Hcompat : compat_memM m2 ((x, eiM_lazy t2 (map fst cenv)) :: m2)) by admit.
+      specialize (IHredM ((x, clo_term t2 (map snd cenv)) :: xvs) (extE_term t1)).
+      destruct IHredM as (o2 & HredE & Ho2).
+      * reflexivity.
+      * intros y c [[=<- <-] | Hyc]; [|eapply Hcompat, H7; assumption].
+        eapply read_eiM_lazy; simpl; [rewrite freevar_eq_dec_eq_ifte; reflexivity|].
+        intros y c Hyc; apply Hcompat, H8, Henv2; assumption.
+      * constructor.
+      * exists o2. split; [|eapply compat_memM_read_outM, compat_memM_read_outM; eassumption].
+        constructor. simpl in *. destruct t2; try assumption.
+        rewrite nth_error_map in *; destruct nth_error; [congruence|assumption].
+  - inversion H3; unexistT; subst; simpl in *.
+    eexists; split; [econstructor|]. constructor.
+  - inversion H3; unexistT; subst; simpl in *.
+    inversion H7; unexistT; subst; simpl in *.
+    eexists; split; [econstructor|].
+    constructor; [assumption|]. apply read_valM_nf.
+Qed.
+
+
+
+
+
+
+
+
+
+
+
+
+
+
+
+
+
+
+
+
+
+
+
+
+
+
+
+
+
+
+
+
